Add1sp1 proof except overflow

code/mpfr/MPFR.Add1sp1.Lemma.fst
@@ -12,26 +12,206 @@ open MPFR.Lib
 open MPFR.Lib.Spec
 open MPFR.Add1.Spec
 open MPFR.Round.Spec
+open MPFR.Dyadic
 open MPFR.Maths
 
 module I64 = FStar.Int64
 module I32 = FStar.Int32
 module U32 = FStar.UInt32
 
-#set-options "--z3refresh --z3rlimit 80 --max_fuel 1 --initial_fuel 0 --max_ifuel 1 --initial_ifuel 0"
+#set-options "--z3refresh --z3rlimit 100 --max_fuel 1 --initial_fuel 0 --max_ifuel 1 --initial_ifuel 0"
+
+(* Rounding lemmas *)
+val mpfr_add1sp1_is_even_lemma: a0:mp_limb_t -> sh:mpfr_prec_t{U32.v sh > 0 /\ U32.v sh < 64} ->
+    high:normal_fp{high.len >= 64 /\ high.prec = 64 - U32.v sh} -> Lemma
+    (requires (v a0 * pow2 (high.len - 64) = high.limb))
+    (ensures  (is_even high = ((a0 &^ (mpfr_LIMB_ONE <<^ sh)) =^ 0uL)))
+
+let mpfr_add1sp1_is_even_lemma a0 sh high =
+    let p = 64 - U32.v sh in
+    lemma_multiple_div (v a0) (pow2 (high.len - 64));
+    assert(v a0 = high.limb / pow2 (high.len - 64));
+    lemma_pow2_div_range high.limb (high.len - 64) high.len;
+    slice_left_nth_lemma #high.len high.limb 64;
+    assert(UInt.nth (v a0) p = UInt.nth #high.len high.limb p);
+    let gb = a0 &^ (mpfr_LIMB_ONE <<^ sh) in
+    lemma_pow2_small_mod (U32.v sh) 64;
+    //! assert(v (mpfr_LIMB_ONE <<^ sh) = pow2 (U32.v sh));
+    lemma_bit_mask_value a0 (mpfr_LIMB_ONE <<^ sh) (p - 1)
+
+let mpfr_add1sp1_round_spec (high:normal_fp) (rb:bool) (sb:bool) (rnd_mode:mpfr_rnd_t):
+    Tot (r:normal_fp{r.prec = high.prec}) =
+    if rb = false && sb = false then high
+    else if MPFR_RNDN? rnd_mode then begin
+	if rb = false || (sb = false && is_even high)
+	then high
+	else add_one_ulp high
+    end else if mpfr_IS_LIKE_RNDZ rnd_mode (high.sign = -1) then high
+    else add_one_ulp high
+
+val mpfr_round_spec_lemma:
+    high1:normal_fp ->
+    high2:normal_fp{high1.prec = high2.prec /\ eval high1 =. eval high2} ->
+    rb:bool -> sb:bool -> rnd_mode:mpfr_rnd_t -> Lemma
+    (eval (mpfr_add1sp1_round_spec high1 rb sb rnd_mode) =.
+     eval (mpfr_add1sp1_round_spec high2 rb sb rnd_mode))
+
+let mpfr_round_spec_lemma high1 high2 rb sb rnd_mode =
+    eval_eq_reveal_lemma high1 high2;
+    eval_eq_intro_lemma (add_one_ulp high1) (add_one_ulp high2)
+
+val mpfr_round_rb_sb_lemma_: a:normal_fp -> p:pos{p < a.prec} ->
+    high:normal_fp{high == high_mant a p} ->
+    rb:bool{rb = rb_def a p} -> sb:bool{sb = sb_def a p} -> rnd_mode:mpfr_rnd_t -> Lemma
+    (mpfr_add1sp1_round_spec high rb sb rnd_mode == round_def a p rnd_mode)
+    
+let mpfr_round_rb_sb_lemma_ a p high rb sb rnd_mode = rb_sb_lemma a p
+
+val mpfr_round_rb_sb_lemma: a:normal_fp -> p:pos{p < a.prec} ->
+    high:normal_fp{high.prec = p /\ eval high =. eval (high_mant a p)} ->
+    rb:bool{rb = rb_def a p} -> sb:bool{sb = sb_def a p} -> rnd_mode:mpfr_rnd_t -> Lemma
+    (eval (mpfr_add1sp1_round_spec high rb sb rnd_mode) =. eval (round_def a p rnd_mode))
+    
+let mpfr_round_rb_sb_lemma a p high rb sb rnd_mode =
+    mpfr_round_rb_sb_lemma_ a p (high_mant a p) rb sb rnd_mode;
+    mpfr_round_spec_lemma high (high_mant a p) rb sb rnd_mode
+
+val mpfr_round_cond_lemma_: a:normal_fp -> p:pos{p < a.prec /\ mpfr_PREC_COND p} ->
+    high:normal_fp{high.prec = p /\ eval high =. eval (high_mant a p)} ->
+    rb:bool{rb = rb_def a p} -> sb:bool{sb = sb_def a p} -> rnd_mode:mpfr_rnd_t ->
+    r:mpfr_fp{r.prec = p} -> Lemma
+    (requires (normal_to_mpfr_cond (mpfr_add1sp1_round_spec high rb sb rnd_mode) r))
+    (ensures  (normal_to_mpfr_cond (round_def a p rnd_mode) r))
+
+let mpfr_round_cond_lemma_ a p high rb sb rnd_mode r =
+    mpfr_round_rb_sb_lemma a p high rb sb rnd_mode;
+    eval_eq_reveal_lemma (mpfr_add1sp1_round_spec high rb sb rnd_mode) (round_def a p rnd_mode)
+    
+val mpfr_round_cond_lemma: a:normal_fp -> p:pos{p < a.prec /\ mpfr_PREC_COND p} ->
+    high:normal_fp{high.prec = p /\ high.sign = (high_mant a p).sign /\
+                   high.exp = (high_mant a p).exp /\ high.len <= (high_mant a p).len /\
+		   high.limb * pow2 (a.len - high.len) = (high_mant a p).limb} ->
+    rb:bool{rb = rb_def a p} -> sb:bool{sb = sb_def a p} -> rnd_mode:mpfr_rnd_t ->
+    r:mpfr_fp{r.prec = p} -> Lemma
+    (requires (normal_to_mpfr_cond (mpfr_add1sp1_round_spec high rb sb rnd_mode) r))
+    (ensures  (normal_to_mpfr_cond (round_def a p rnd_mode) r))
+
+let mpfr_round_cond_lemma a p high rb sb rnd_mode r =
+    assert(eval_abs high =. eval_abs (high_mant a p));
+    mpfr_round_cond_lemma_ a p high rb sb rnd_mode r
+
+let mpfr_add1sp1_ternary_spec (high:normal_fp) (rb:bool) (sb:bool) (rnd_mode:mpfr_rnd_t):
+    Tot int =
+    if rb = false && sb = false then 0
+    else if MPFR_RNDN? rnd_mode then begin
+	if rb = false || (sb = false && is_even high)
+	then -high.sign
+	else high.sign
+    end else if mpfr_IS_LIKE_RNDZ rnd_mode (high.sign = -1) then -high.sign
+    else high.sign
+    
+val mpfr_truncate_ternary_cond_lemma: a:normal_fp{mpfr_EXP_COND a.exp} ->
+    p:pos{p < a.prec /\ mpfr_PREC_COND p} ->
+    high:normal_fp{high.prec = p /\ eval high =. eval (high_mant a p)} ->
+    rb:bool{rb = rb_def a p} -> sb:bool{sb = sb_def a p} -> rnd_mode:mpfr_rnd_t ->
+    f:int -> r:mpfr_fp{r.prec = p} -> Lemma
+    (requires (normal_to_mpfr_cond high r /\
+               f = (if rb = false && sb = false then 0 else -a.sign)))
+    (ensures  (mpfr_ternary_cond f a r))
+
+let mpfr_truncate_ternary_cond_lemma a p high rb sb rnd_mode f r =
+    eval_eq_reveal_lemma high (high_mant a p);
+    mpfr_overflow_bound_lemma high;
+    mpfr_underflow_bound_lemma high;
+    normal_to_mpfr_cond_in_range_lemma high r;
+    rb_sb_lemma a p;
+    if rb = false && sb = false then eval_eq_intro_lemma a (high_mant a p)
+    else if a.sign = 1 then eval_lt_intro_lemma (high_mant a p) a
+    else eval_lt_intro_lemma a (high_mant a p)
+
+val mpfr_add_one_ulp_ternary_cond_lemma: a:normal_fp{mpfr_EXP_COND a.exp} ->
+    p:pos{p < a.prec /\ mpfr_PREC_COND p} ->
+    high:normal_fp{high.prec = p /\ eval high =. eval (high_mant a p)} -> rnd_mode:mpfr_rnd_t ->
+    f:int -> r:mpfr_fp{r.prec = p} -> Lemma
+    (requires (normal_to_mpfr_cond (add_one_ulp high) r /\
+               f = a.sign))
+    (ensures  (mpfr_ternary_cond f a r))
+
+let mpfr_add_one_ulp_ternary_cond_lemma a p high rnd_mode f r =
+    eval_eq_reveal_lemma high (high_mant a p);
+    mpfr_overflow_bound_lemma high;
+    mpfr_underflow_bound_lemma high;
+    if mpfr_overflow_bound p >. eval_abs high then begin
+        add_one_ulp_lt_lemma (mpfr_max_value 1 p) high;
+	normal_to_mpfr_cond_in_range_lemma (add_one_ulp high) r;
+	if a.sign = 1 then eval_lt_intro_lemma a (add_one_ulp high)
+	else eval_lt_intro_lemma (add_one_ulp high) a
+    end else begin
+        assert(mpfr_overflow_bound p =. eval_abs high)
+    end
+
+val mpfr_ternary_cond_lemma_: a:normal_fp{mpfr_EXP_COND a.exp} ->
+    p:pos{p < a.prec /\ mpfr_PREC_COND p} ->
+    high:normal_fp{high.prec = p /\ eval high =. eval (high_mant a p)} ->
+    rb:bool{rb = rb_def a p} -> sb:bool{sb = sb_def a p} -> rnd_mode:mpfr_rnd_t ->
+    f:int -> r:mpfr_fp{r.prec = p} -> Lemma
+    (requires (normal_to_mpfr_cond (mpfr_add1sp1_round_spec high rb sb rnd_mode) r /\
+               f = mpfr_add1sp1_ternary_spec high rb sb rnd_mode))
+    (ensures  (mpfr_ternary_cond f a r))
+
+let mpfr_ternary_cond_lemma_ a p high rb sb rnd_mode f r =
+    if rb = false && sb = false then mpfr_truncate_ternary_cond_lemma a p high rb sb rnd_mode f r
+    else if MPFR_RNDN? rnd_mode then begin
+	if rb = false || (sb = false && is_even high)
+	then mpfr_truncate_ternary_cond_lemma a p high rb sb rnd_mode f r
+	else mpfr_add_one_ulp_ternary_cond_lemma a p high rnd_mode f r
+    end else if mpfr_IS_LIKE_RNDZ rnd_mode (high.sign = -1) then
+        mpfr_truncate_ternary_cond_lemma a p high rb sb rnd_mode f r
+    else mpfr_add_one_ulp_ternary_cond_lemma a p high rnd_mode f r
+
+val mpfr_ternary_cond_lemma: a:normal_fp{mpfr_EXP_COND a.exp} ->
+    p:pos{p < a.prec /\ mpfr_PREC_COND p} ->
+    high:normal_fp{high.prec = p /\ high.sign = (high_mant a p).sign /\
+                   high.exp = (high_mant a p).exp /\ high.len <= (high_mant a p).len /\
+		   high.limb * pow2 (a.len - high.len) = (high_mant a p).limb} ->
+    rb:bool{rb = rb_def a p} -> sb:bool{sb = sb_def a p} -> rnd_mode:mpfr_rnd_t ->
+    f:int -> r:mpfr_fp{r.prec = p} -> Lemma
+    (requires (normal_to_mpfr_cond (mpfr_add1sp1_round_spec high rb sb rnd_mode) r /\
+               f = mpfr_add1sp1_ternary_spec high rb sb rnd_mode))
+    (ensures  (mpfr_ternary_cond f a r))
+
+let mpfr_ternary_cond_lemma a p high rb sb rnd_mode f r =
+    assert(eval_abs high =. eval_abs (high_mant a p));
+    mpfr_ternary_cond_lemma_ a p high rb sb rnd_mode f r
+
+val mpfr_add1sp1_post_cond_lemma: a:normal_fp{mpfr_EXP_COND a.exp} ->
+    p:pos{p < a.prec /\ mpfr_PREC_COND p} ->
+    high:normal_fp{high.prec = p /\ high.sign = (high_mant a p).sign /\
+                   high.exp = (high_mant a p).exp /\ high.len <= (high_mant a p).len /\
+		   high.limb * pow2 (a.len - high.len) = (high_mant a p).limb} ->
+    rb:bool{rb = rb_def a p} -> sb:bool{sb = sb_def a p} -> rnd_mode:mpfr_rnd_t ->
+    f:int -> r:mpfr_fp{r.prec = p} -> Lemma
+    (requires (normal_to_mpfr_cond (mpfr_add1sp1_round_spec high rb sb rnd_mode) r /\
+               f = mpfr_add1sp1_ternary_spec high rb sb rnd_mode))
+    (ensures  (mpfr_round_cond a p rnd_mode r /\
+               mpfr_ternary_cond f a r))
+
+let mpfr_add1sp1_post_cond_lemma a p high rb sb rnd_mode f r =
+    mpfr_round_cond_lemma a p high rb sb rnd_mode r;
+    mpfr_ternary_cond_lemma a p high rb sb rnd_mode f r
 
 (* intermediate results *)
 private type mpfr_tmp_exp_t = x:mpfr_exp_t{I32.(x >=^ mpfr_EMIN /\ x <=^ mpfr_EMAX +^ 1l)}
 
 (* pre/post-condition for mpfr_add1sp1_any *)
-let mpfr_add1sp1_common_pre_cond a b c (p:mpfr_reg_prec_t) h =
+let mpfr_add1sp1_common_pre_cond a b c (p:mpfr_prec_t) h =
     mpfr_reg_cond_ h b /\ mpfr_reg_cond_ h c /\
-    U32.v p < U32.v gmp_NUMB_BITS /\
+    0 < U32.v p /\ U32.v p < U32.v gmp_NUMB_BITS /\
     a.mpfr_prec = p /\ b.mpfr_prec = p /\ c.mpfr_prec = p /\
     live h a.mpfr_d /\ live h b.mpfr_d /\ live h c.mpfr_d /\
     length a.mpfr_d = 1 /\ length b.mpfr_d = 1 /\ length c.mpfr_d = 1
 
-let mpfr_add1sp1_any_pre_cond a b c (p:mpfr_reg_prec_t) h =
+let mpfr_add1sp1_any_pre_cond a b c (p:mpfr_prec_t) h =
     a.mpfr_sign = b.mpfr_sign /\
     mpfr_add1sp1_common_pre_cond a b c p h
     
@@ -177,8 +357,7 @@ let mpfr_add1sp1_gt_branch12_rb_lemma h a b c sh d mask =
     let a0 = b0 +%^ (c0 >>^ d) in
     let a0 = if a0 <^ b0 then mpfr_LIMB_HIGHBIT |^ (a0 >>^ 1ul) else a0 in
     mpfr_add1sp1_gt_branch12_a0_bx_lemma h a b c sh d mask;
-    //! assert(v a0 * pow2 (r.len - 64) = r.limb);
-    lemma_multiple_div (v a0) (pow2 (r.len - 64));
+    //! assert(v a0 = r.limb / pow2 (r.len - 64));
     UInt.slice_left_lemma (UInt.to_vec #r.len r.limb) 64;
     //! assert(UInt.nth (v a0) p = UInt.nth #r.len r.limb p);
     let rb = a0 &^ (mpfr_LIMB_ONE <<^ U32.(sh -^ 1ul)) in
@@ -186,7 +365,7 @@ let mpfr_add1sp1_gt_branch12_rb_lemma h a b c sh d mask =
     //! assert(v (mpfr_LIMB_ONE <<^ U32.(sh -^ 1ul)) = pow2 (U32.v sh - 1));
     lemma_bit_mask_value a0 (mpfr_LIMB_ONE <<^ U32.(sh -^ 1ul)) p
 
-val mpfr_add1sp1_gt_branch12_latter_sb_lemma:
+val mpfr_add1sp1_gt_branch12_former_sb_lemma:
     h:mem -> a:mpfr_struct -> b:mpfr_struct -> c:mpfr_struct ->
     sh:mpfr_reg_prec_t -> d:u32 -> mask:mp_limb_t -> Lemma
     (requires (mpfr_add1sp1_gt_branch1_pre_cond a b c sh d mask h \/
@@ -204,7 +383,7 @@ val mpfr_add1sp1_gt_branch12_latter_sb_lemma:
     let sb = (a0 &^ mask) ^^ rb in
     v sb = r.limb % pow2 (r.len - p - 1) / pow2 (r.len - 64)))
 
-let mpfr_add1sp1_gt_branch12_latter_sb_lemma h a b c sh d mask =
+let mpfr_add1sp1_gt_branch12_former_sb_lemma h a b c sh d mask =
     let p = U32.v a.mpfr_prec in
     let r = add1sp_exact (as_reg_fp_ h b) (as_reg_fp_ h c) in
     let bp = b.mpfr_d in
@@ -264,13 +443,13 @@ let mpfr_add1sp1_gt_branch1_sb_lemma h a b c sh d mask =
     //! assert(v c0 % pow2 (r.len - 64) = 0);
     lemma_mod_distr_zero (v b0 * pow2 (U32.v d)) (v c0) (pow2 (r.len - 64));
     //! assert(r.limb % pow2 (r.len - 64) = 0);
-    mpfr_add1sp1_gt_branch12_latter_sb_lemma h a b c sh d mask;
+    mpfr_add1sp1_gt_branch12_former_sb_lemma h a b c sh d mask;
     lemma_pow2_mod_mod r.limb (r.len - p - 1) (r.len - 64);
     lemma_div_mul (r.limb % pow2 (r.len - p - 1)) (pow2 (r.len - 64));
     //! assert(v sb * pow2 (r.len - 64) = r.limb % pow2 (r.len - p - 1));
     lemma_mul_zero (v sb) (pow2 (r.len - 64))
 
-val mpfr_add1sp1_gt_branch2_init_sb_lemma:
+val mpfr_add1sp1_gt_branch2_latter_sb_lemma:
     h:mem -> a:mpfr_struct -> b:mpfr_struct -> c:mpfr_struct ->
     sh:mpfr_reg_prec_t -> d:u32 -> mask:mp_limb_t -> Lemma
     (requires (mpfr_add1sp1_gt_branch2_pre_cond a b c sh d mask h))
@@ -284,7 +463,7 @@ val mpfr_add1sp1_gt_branch2_init_sb_lemma:
     let a0 = b0 +%^ (c0 >>^ d) in
     (v sb <> 0) = (r.limb % pow2 (U32.v d) <> 0)))
 
-let mpfr_add1sp1_gt_branch2_init_sb_lemma h a b c sh d mask =
+let mpfr_add1sp1_gt_branch2_latter_sb_lemma h a b c sh d mask =
     let r = add1sp_exact (as_reg_fp_ h b) (as_reg_fp_ h c) in
     let bp = b.mpfr_d in
     let cp = c.mpfr_d in
@@ -331,7 +510,7 @@ let mpfr_add1sp1_gt_branch2_sb_lemma h a b c sh d mask =
     let b0 = Seq.index (as_seq h bp) 0 in
     let c0 = Seq.index (as_seq h cp) 0 in
     let sb = c0 <<^ U32.(gmp_NUMB_BITS -^ d) in
-    mpfr_add1sp1_gt_branch2_init_sb_lemma h a b c sh d mask;
+    mpfr_add1sp1_gt_branch2_latter_sb_lemma h a b c sh d mask;
     let a0 = b0 +%^ (c0 >>^ d) in
     lemma_add_div (v c0) (v b0) (pow2 (U32.v d));
     lemma_pow2_mod_mod (v b0 + v c0 / pow2 (U32.v d)) 64 1;
@@ -349,7 +528,7 @@ let mpfr_add1sp1_gt_branch2_sb_lemma h a b c sh d mask =
     //! assert((r.limb % pow2 (r.len - 64) <> 0) = (v sb <> 0));
     let rb = a0 &^ (mpfr_LIMB_ONE <<^ U32.(sh -^ 1ul)) in
     let sb' = (a0 &^ mask) ^^ rb in
-    mpfr_add1sp1_gt_branch12_latter_sb_lemma h a b c sh d mask;
+    mpfr_add1sp1_gt_branch12_former_sb_lemma h a b c sh d mask;
     lemma_pow2_mod_div r.limb (r.len - p - 1) (r.len - 64);
     //! assert((r.limb / pow2 (r.len - 64) % pow2 (U32.v sh - 1) <> 0) = (v sb' <> 0));
     lemma_sb_logor #r.len r.limb (r.len - p - 1) (r.len - 64) sb sb'
@@ -536,7 +715,7 @@ let mpfr_add1sp1_eq_value_lemma h a b c sh =
     //! assert(v a0 >= pow2 63);
     ()
 
-(* exact the same as mpfr_add1sp1_gt_branch1_rb_lemma *)
+(* exact the same as mpfr_add1sp1_gt_branch12_rb_lemma *)
 val mpfr_add1sp1_eq_rb_sb_lemma:
     h:mem -> a:mpfr_struct -> b:mpfr_struct -> c:mpfr_struct ->
     sh:mpfr_reg_prec_t -> Lemma
